---
layout: post
title: 77. Combinations
---
### Question
Given two integers _n_ and _k_ , return all possible combinations of _k_
numbers out of 1 ... _n_.

 **Example:**

    
    
     **Input:**  n = 4, k = 2
    **Output:**
    [
      [2,4],
      [3,4],
      [2,3],
      [1,2],
      [1,3],
      [1,4],
    ]
    

### Solution 1
    
    
        public static List<List<Integer>> combine(int n, int k) {
    		List<List<Integer>> combs = new ArrayList<List<Integer>>();
    		combine(combs, new ArrayList<Integer>(), 1, n, k);
    		return combs;
    	}
    	public static void combine(List<List<Integer>> combs, List<Integer> comb, int start, int n, int k) {
    		if(k==0) {
    			combs.add(new ArrayList<Integer>(comb));
    			return;
    		}
    		for(int i=start;i<=n;i++) {
    			comb.add(i);
    			combine(combs, comb, i+1, n, k-1);
    			comb.remove(comb.size()-1);
    		}
    	}


### Solution 2
    
    
    class Solution {
    public:
    	vector<vector<int>> combine(int n, int k) {
    		vector<vector<int>> result;
    		int i = 0;
    		vector<int> p(k, 0);
    		while (i >= 0) {
    			p[i]++;
    			if (p[i] > n) --i;
    			else if (i == k - 1) result.push_back(p);
    			else {
    			    ++i;
    			    p[i] = p[i - 1];
    			}
    		}
    		return result;
    	}
    };


### Solution 3
Basically, this solution follows the idea of the mathematical formula
C(n,k)=C(n-1,k-1)+C(n-1,k).

Here C(n,k) is divided into two situations. Situation one, number n is
selected, so we only need to select k-1 from n-1 next. Situation two, number n
is not selected, and the rest job is selecting k from n-1.

    
    
    public class Solution {
        public List<List<Integer>> combine(int n, int k) {
            if (k == n || k == 0) {
                List<Integer> row = new LinkedList<>();
                for (int i = 1; i <= k; ++i) {
                    row.add(i);
                }
                return new LinkedList<>(Arrays.asList(row));
            }
            List<List<Integer>> result = this.combine(n - 1, k - 1);
            result.forEach(e -> e.add(n));
            result.addAll(this.combine(n - 1, k));
            return result;
        }
    }



