---
layout: post
title: 1070. Convert to Base -2
---
### Question
Given a number `N`, return a string consisting of `"0"`s and `"1"`s that
represents its value in base `**-2**` (negative two).

The returned string must have no leading zeroes, unless the string is `"0"`.



 **Example 1:**

    
    
     **Input:** 2
    **Output:** "110"
    **Explantion:** (-2) ^ 2 + (-2) ^ 1 = 2
    

**Example 2:**

    
    
    **Input:** 3
    **Output:** "111"
    **Explantion:** (-2) ^ 2 + (-2) ^ 1 + (-2) ^ 0 = 3
    

**Example 3:**

    
    
    **Input:** 4
    **Output:** "100"
    **Explantion:** (-2) ^ 2 = 4
    



 **Note:**

  1. `0 <= N <= 10^9`

### Solution 1
Please follow more detailed explanation in Chinese here:  
[Youtube](https://www.youtube.com/watch?v=ia_vwGMAFVY&t=6s)  
[Bilibili](https://www.bilibili.com/video/av51966443)

##  **Intuition** :

  1. Maybe write a base2 function first?
  2. How about add minus `-`?
  3. Done.

  

##  **Explanation** :

base2 function is quite basis of basis.  
check last digit, shift to right.  
base-2 is totally no difference, just add a sign `-`.  
  

##  **Time Complexity** :

`O(logN)` Time, `O(logN)` space.  
Note that I didn't deal with string concatenation,  
and just take this part as `O(1)`.

Instead of create a new string each time,  
we can improve this process using some operations join/reverse or data
structure list/vector .  
Like Java we may need `StringBuilder`,  
but those are not what I want to discuss deeply here.

  

##  **Iterative Solution**

 **Java**

    
    
         public String base2(int N) {
            StringBuilder res = new StringBuilder();
            while (N != 0) {
                res.append(N & 1);
                N = N >> 1;
            }
            return res.length() > 0 ? res.reverse().toString() : "0";
        }
    
        public String baseNeg2(int N) {
            StringBuilder res = new StringBuilder();
            while (N != 0) {
                res.append(N & 1);
                N = -(N >> 1);
            }
            return res.length() > 0 ? res.reverse().toString() : "0";
        }
    

**C++**

    
    
         string base2(int N) {
            string res = "";
            while (N) {
                res = to_string(N & 1) + res;
                N = N >> 1;
            }
            return res == ""  ? "0" : res;
        }
    
        string baseNeg2(int N) {
            string res = "";
            while (N) {
                res = to_string(N & 1) + res;
                N = -(N >> 1);
            }
            return res == "" ? "0" : res;
        }
    

**Python**

    
    
         def base2(self, x):
            res = []
            while x:
                res.append(x & 1)
                x = x >> 1
            return "".join(map(str, res[::-1] or [0]))
    
        def baseNeg2(self, x):
            res = []
            while x:
                res.append(x & 1)
                x = -(x >> 1)
            return "".join(map(str, res[::-1] or [0]))
    

  

## **Recursive Solution**

**Java:**

    
    
        public String base2( int N) {
            if (N == 0 || N == 1) return Integer.toString(N);
            return base2(N >> 1) + Integer.toString(N & 1);
        }
    
        public String baseNeg2(int N) {
            if (N == 0 || N == 1) return Integer.toString(N);
            return baseNeg2(-(N >> 1)) + Integer.toString(N & 1);
        }
    

**C++:**

    
    
         string base2(int N) {
            if (N == 0 || N == 1) return to_string(N);
            return base2(N >> 1) + to_string(N & 1);
        }
    
        string baseNeg2(int N) {
            if (N == 0 || N == 1) return to_string(N);
            return baseNeg2(-(N >> 1)) + to_string(N & 1);
        }
    

**Python:**

    
    
         def base2(self, N):
            if N == 0 or N == 1: return str(N)
            return self.base2(N >> 1) + str(N & 1)
    
        def baseNeg2(self, N):
            if N == 0 or N == 1: return str(N)
            return self.baseNeg2(-(N >> 1)) + str(N & 1)
    

  

## More

[Easy One Line](https://leetcode.com/problems/convert-to-
base-2/discuss/287017/JavaPython-Easy-One-Line)


### Solution 2
for each number, we first consider its binary mode, then we check
10,1000,100000,... one by one  
for example, 6 = '110', so for the second '1', in base -2, it makes the
initial number decrease `4(+2 -> -2)`  
so we jusr make the initial number add 4, then 6 -> 10 = '1010', later we
consider the first '1', it makes the initial number decrease `16(+8 -> -8)`,
then we add 16, 10 -> 26 = '11010', now we get the answer.

    
    
    class Solution:
        def baseNeg2(self, N: int) -> str:
            neg = [1 << i for i in range(1, 33, 2)]
            for mask in neg:
                if N & mask: N += mask*2
            return bin(N)[2:]
    


### Solution 3
See this Geeks4Geeks article: [Convert a number into negative base
representation](https://www.geeksforgeeks.org/convert-number-negative-base-
representation/).

Below is the specialized solution for the `-2` base.

    
    
    string baseNeg2(int N, string res = "") {
      while (N != 0) {
        int rem = N % -2;
        N /= -2;
        if (rem < 0) rem += 2, N += 1;
        res = to_string(rem) + res;
      }
      return max(string("0"), res);
    }
    



